crypto/bignum/x25519/Hacl.Bignum.Crecip.fst
@@ -6,15 +6,20 @@ open FStar.Buffer
 open Hacl.Bignum.Parameters
 open Hacl.Spec.Bignum.Bigint
 open Hacl.Bignum.Limb
+open Hacl.Bignum.Fsquare
 open Hacl.Bignum.Fmul
 
+
+#set-options "--initial_fuel 0 --max_fuel 0 --z3rlimit 100"
 #set-options "--lax"
 
 val crecip:
   out:felem ->
-  z:felem -> Stack unit
-  (requires (fun h -> live h out /\ live h z))
-  (ensures (fun h0 _ h1 -> live h1 out /\ modifies_1 out h0 h1))
+  z:felem{disjoint out z} ->
+  Stack unit
+  (requires (fun h -> live h out /\ live h z /\ Hacl.Spec.EC.AddAndDouble.red_513 (as_seq h z)))
+  (ensures (fun h0 _ h1 -> live h1 out /\ modifies_1 out h0 h1
+    /\ Hacl.Spec.EC.AddAndDouble.red_513 (as_seq h1 out)))
 let crecip out z =
   push_frame();
   let buf = create limb_zero 20ul in
