crypto/bignum/x25519/Hacl.Spec.Bignum.Crecip.fst
@@ -1,0 +1,38 @@
+module Hacl.Spec.Bignum.Crecip
+
+open Hacl.Bignum.Parameters
+open Hacl.Spec.Bignum.Bigint
+open Hacl.Bignum.Limb
+open Hacl.Spec.Bignum.Fsquare
+open Hacl.Spec.Bignum
+open Hacl.Spec.EC.AddAndDouble
+
+
+#set-options "--initial_fuel 0 --max_fuel 0 --z3rlimit 10"
+#set-options "--lax"
+
+val crecip:
+  z:seqelem{red_513 z} -> Tot (s':seqelem{red_513 s'})
+let crecip z =
+  let a = fsquare_times_tot z 1 in
+  let t0 = fsquare_times_tot a 2 in
+  let b = fmul_tot t0 z in
+  let a' = fmul_tot b a in
+  let t0' = fsquare_times_tot a 1 in
+  let b' = fmul_tot t0' b in
+  let t0'' = fsquare_times_tot b' 5 in
+  let b'' = fmul_tot t0'' b' in
+  let t0''' = fsquare_times_tot b'' 10 in
+  let c = fmul_tot t0''' b'' in
+  let t0'''' = fsquare_times_tot c 20 in
+  let t0''''' = fmul_tot t0'''' c in
+  let t0_6 = fsquare_times_tot t0''''' 10 in
+  let b''' = fmul_tot t0_6 b'' in
+  let t0_7 = fsquare_times_tot b''' 50 in
+  let c' = fmul_tot t0_7 b''' in
+  let t0_8 = fsquare_times_tot c' 100 in
+  let t0_9 = fmul_tot t0_8 c' in
+  let t0_10 = fsquare_times_tot t0_9 50 in
+  let t0_11 = fmul_tot t0_10 b''' in
+  let t0_12 = fsquare_times_tot t0_11 5 in
+  fmul_tot t0_12 a'
